# 实现 add(1)(2)(3) 等于 6

```js
function add (num) {
  let sum = num
  const add = n => {
    sum = sum + n
    return add
  }
  add.toString = () => sum
  return add
}
```

## 变种add(1)(2, 3) 等于 6

```js
function add () {
	let sum = 0
	function add () {
		for (let i = 0; i < arguments.length; i++) {
			sum += +arguments[i]
		}
		return add
	}
	add.valueOf = function () {
		return sum
	}
	return add.apply(null, arguments)
}

function add (...args) {
	var fn = function (...params) {
		return add.apply(this, [...args, ...params])
	}
	fn.toString = function () {
		return Array.prototype.reduce.call(args, function (total, curr) {
			return total + curr
		}, 0)
	}
	return fn
}

function add () {
   var args = Array.prototype.slice.call(arguments)
   var fn = function () {
      args.push(...arguments)
      return fn
   }

	fn.valueOf = function () {
		return args.reduce(function (a, b) {
			return a + b
		})
  }

  return fn
}

function add(a, b) { return (a = add.bind(0, b = [].join.call(arguments, '+'))).toString = eval.bind(0, b), a }

+add()
```